thys/Superposition_Calculus/Superposition.thy
@@ -304,6 +304,4 @@ qed
 
 end
 
-
-
 end
